Find (\textit{a}) $v_2$, (\textit{b}) $v_1$, (\textit{c}) $i_4$; from Fig. 1-66.
\begin{enumerate}[leftmargin=2cm,labelsep=.5cm,label=\bfseries\alph*)]
\item $
\begin{aligned}[t]
R_{eq_{v2}} &= R_2\parallel (R_3+R_4) \\
&= \frac{R_2(R_3+R_4)}{R_2+R_3+R_4} \\[5mm]
v_2 &= \hlbox{$V_s\left(\frac{R_2\parallel (R_3+R_4)}{R_1 + R_2\parallel (R_3+R_4)}\right)$} 
\end{aligned} $ 
\\[1cm]

\item $
\begin{aligned}[t]
v_1 &= V_s-v_2 \\[5mm]
&= \hlbox{$V_s\left(\frac{R_1(R_2+R_3+R_4)}{R_2\parallel (R_3+R_4)}\right)$} 
\end{aligned} $
\\[1cm]

\item $
\begin{aligned}[t]
i_4&= \hlbox{$V_s\left(\frac{V_s(R_2)}{R_2\parallel (R_3+R_4)}\right)$} 
\end{aligned} $
\\[1cm]

\end{enumerate}